example/Fir.Check.fst
@@ -2,6 +2,7 @@
 module Fir.Check
 
 open Pipit.Sugar.Vanilla
+module Check = Pipit.Sugar.Check
 
 // open Pipit.System.Base
 open Pipit.System.Ind
@@ -20,29 +21,20 @@ let rec fir (coeffs: list R.real) (input: reals): reals =
 
 let fir2 (input: reals): reals = fir [0.7R; 0.3R] input
 
-let bibo2 (n: pos) (signal: reals): bools =
+let bibo2_body (n: pos) (signal: reals): bools =
   check "bibo" (sofar (abs signal <=^ pure n) => (abs (fir2 signal) <=^ pure n))
 
-let bibo2' n =
-  assert_norm (Pipit.Exp.Causality.causal (run1 (bibo2 n)));
-  system_of_exp (run1 (bibo2 n))
-
-let proof2 (n: pos): Lemma (ensures induct1 (bibo2' n)) =
-  assert (base_case (bibo2' n)) by (T.pipit_simplify ());
-  assert (step_case (bibo2' n)) by (T.pipit_simplify ());
-  ()
+let bibo2 n: reals -> bools =
+  let e = Check.exp_of_stream1 (bibo2_body n) in
+  assert (Check.system_induct_k1 e) by (T.norm_full ());
+  Check.stream_of_checked1 e
 
 let fir3 (input: reals): reals = fir [0.7R; 0.2R; 0.1R] input
 
-let bibo3 (n: pos) (signal: reals): bools =
+let bibo3_body (n: pos) (signal: reals): bools =
   check "bibo" (sofar (abs signal <=^ pure n) => (abs (fir3 signal) <=^ pure n))
 
-let bibo3' n =
-  assert_norm (Pipit.Exp.Causality.causal (run1 (bibo3 n)));
-  system_of_exp (run1 (bibo3 n))
-
-let proof3 (n: pos): Lemma (ensures induct_k 2 (bibo3' n)) =
-  assert (base_case_k 2 (bibo3' n)) by (T.pipit_simplify ());
-  assert (step_case_k 2 (bibo3' n)) by (T.pipit_simplify ());
-  ()
-
+let bibo3 n: reals -> bools =
+  let e = Check.exp_of_stream1 (bibo3_body n) in
+  assert (Check.system_induct_k 2 e) by (T.norm_full ());
+  Check.stream_of_checked1 e
