example/Simple.Check.fst
@@ -6,7 +6,12 @@ open Pipit.System.Ind
 open Pipit.System.Exp
 
 module T = Pipit.Tactics
+
 open Pipit.Sugar.Vanilla
+module Base = Pipit.Sugar.Base
+module Check = Pipit.Sugar.Check
+
+module Vanilla = Pipit.Prim.Vanilla
 
 (*
    Count the number of times a predicate has been true.
@@ -22,7 +27,7 @@ let count_when (p: bools): ints =
    fby 0 count +^ (if_then_else p z1 z0))
 
 (* forall e. count_when false <= count_when e <= count_when true *)
-let count_when_prop (e: bools): bools =
+let count_when_prop_body (e: bools): bools =
   let' (count_when ff) (fun count_when_false ->
   let' (count_when  e) (fun count_when_e ->
   let' (count_when tt) (fun count_when_true ->
@@ -31,10 +36,18 @@ let count_when_prop (e: bools): bools =
   check' "count_when e     <= count_when true"  (count_when_e     <=^ count_when_true) (
   pure true))))))
 
-let sys =
-  assert_norm (Pipit.Exp.Causality.causal (run1 count_when_prop));
-  system_of_exp (run1 count_when_prop)
+let count_when_prop: bools -> bools =
+  let e = Check.exp_of_stream1 count_when_prop_body in
+  assert (Check.system_induct_k1 e) by (T.norm_full ());
+  Check.stream_of_checked1 e
 
-let prove (): Lemma (ensures induct1 sys) =
-  assert (base_case sys) by (T.norm_full ());
-  assert (step_case sys) by (T.norm_full ())
+let sum_contract (i: ints): Base._contract Vanilla.table Vanilla.TInt = {
+    rely = i >^ z0;
+    guar = (fun sum -> sum >^ (0 `fby` sum));
+    impl = rec' (fun sum -> (0 `fby` sum) +^ i);
+  }
+
+let sum: ints -> ints =
+  let c = Check.contract_of_stream1 sum_contract in
+  assert (Check.contract_system_induct_k1 c) by (T.norm_full ());
+  Check.stream_of_contract1 c
