src/Pipit.Sugar.Check.fst
@@ -1,0 +1,87 @@
+module Pipit.Sugar.Check
+
+open Pipit.Prim.Table
+
+open Pipit.Exp.Base
+
+open Pipit.Sugar.Base
+module Base = Pipit.Sugar.Base
+
+module XC  = Pipit.Exp.Checked.Base
+module XCC = Pipit.Exp.Checked.Compound
+module PM  = Pipit.Prop.Metadata
+
+// module SB  = Pipit.System.Base
+module SI  = Pipit.System.Ind
+module SX  = Pipit.System.Exp
+
+noeq
+type _contract (t: table) (c: context t) (a: t.ty) = {
+  rely: XCC.cexp t       c  t.propty;
+  guar: XCC.cexp t (a :: c) t.propty;
+  impl: XCC.cexp t       c         a;
+}
+
+let contract_of_stream1 (#t: table) (#a #b: t.ty) (f: s t a -> Base._contract t b) : _contract t [a] b = {
+  rely = exp_of_stream1 (fun a -> (f a).rely);
+  guar = exp_of_stream2 (fun b a -> (f a).guar b);
+  impl = exp_of_stream1 (fun a -> (f a).impl);
+}
+
+
+let contract_system_induct_k1 (#t: table) (#c: context t) (#a: t.ty) (contr: _contract t c a): prop =
+  Pipit.Exp.Causality.causal contr.rely /\
+  Pipit.Exp.Causality.causal contr.guar /\
+  Pipit.Exp.Causality.causal contr.impl /\
+  SI.induct1 (SX.system_of_contract contr.rely contr.guar contr.impl)
+
+
+let stream_of_contract1 (#t: table) (#a #b: t.ty) (contr: _contract t [a] b): s t a -> s t b =
+  let rely = XC.bless contr.rely in
+  let guar = XC.bless contr.guar in
+  let impl = XC.bless contr.impl in
+  // TODO:ADMIT: requires contract_check
+  let e = XContract PM.PSUnknown rely guar impl in
+  assume (XC.check' PM.check_mode_valid e);
+  stream_of_exp1 e
+
+
+let exp_of_stream0 (#t: table) (#ty: t.ty) (e: s t ty) : XCC.cexp t [] ty = exp_of_stream0 e
+let exp_of_stream1 (#t: table) (#a #b: t.ty) (f: s t a -> s t b) : XCC.cexp t [a] b = exp_of_stream1 f
+let exp_of_stream2 (#t: table) (#a #b #c: t.ty) (f: s t a -> s t b -> s t c) : XCC.cexp t [a; b] c = exp_of_stream2 f
+
+
+let stream_of_checked0 (#t: table) (#a: t.ty) (e: exp t [] a { XC.check' PM.check_mode_all e }): s t a =
+  let e' = XC.bless e in
+  stream_of_exp0 e'
+
+let stream_of_checked1 (#t: table) (#a #b: t.ty) (e: exp t [a] b { XC.check' PM.check_mode_all e }): s t a -> s t b =
+  let e' = XC.bless e in
+  stream_of_exp1 e'
+
+let stream_of_checked2 (#t: table) (#a #b #c: t.ty) (e: exp t [a; b] c { XC.check' PM.check_mode_all e }): s t a -> s t b -> s t c =
+  let e' = XC.bless e in
+  stream_of_exp2 e'
+
+
+let system_induct_k1 (#t: table) (#c: context t) (#a: t.ty) (e: XCC.cexp t c a): prop =
+  Pipit.Exp.Causality.causal e /\ SI.induct1 (SX.system_of_exp e)
+
+let system_induct_k (#t: table) (#c: context t) (#a: t.ty) (k: nat) (e: XCC.cexp t c a): prop =
+  Pipit.Exp.Causality.causal e /\ SI.induct_k k (SX.system_of_exp e)
+
+let lemma_check_system_induct_k1 (#t: table) (#c: context t) (#a: t.ty) (e: XCC.cexp t c a):
+  Lemma (requires (system_induct_k1 e))
+        (ensures  (XC.check' PM.check_mode_all e))
+        [SMTPat (system_induct_k1 e)]
+        =
+    // TODO:ADMIT: induction is sound
+    admit ()
+
+let lemma_check_system_induct_k (#t: table) (#c: context t) (#a: t.ty) (k: nat) (e: XCC.cexp t c a):
+  Lemma (requires (system_induct_k k e))
+        (ensures  (XC.check' PM.check_mode_all e))
+        [SMTPat (system_induct_k k e)]
+        =
+    // TODO:ADMIT: induction is sound
+    admit ()
